IMP- to IMP-- tail recursive

Cook_Levin/IMP-_To_SAS+/IMP-_To_IMP--/IMP_Minus_To_IMP_Minus_Minus_nat.thy
@@ -84,37 +84,208 @@ lemma sub_var_bit_list: "var_bit_list_nat n (vname_encode v) = vname_list_encode
 
 
 declare nth_nat.simps[simp del]
-datatype IMPm_IMPmm = SKIP | 
-                      Assign vname aexp |
-                      Seq_0 IMP_Minus_com IMP_Minus_com |
-                      Seq_m IMP_Minus_com IMP_Minus_com IMP_Minus_Minus_com |
-                      Seq_f IMP_Minus_com IMP_Minus_com IMP_Minus_Minus_com IMP_Minus_Minus_com |
-                      If_0  vname IMP_Minus_com IMP_Minus_com |
-                      If_m  vname IMP_Minus_com IMP_Minus_com IMP_Minus_Minus_com |
-                      If_f vname IMP_Minus_com IMP_Minus_com IMP_Minus_Minus_com IMP_Minus_Minus_com |
-                      While_0 vname IMP_Minus_com|
-                      While_f vname IMP_Minus_com IMP_Minus_Minus_com
+datatype IMPm_IMPmm = Bot IMP_Minus_Minus_com |
+                      SKIP nat| 
+                      Assign vname aexp nat |
+                      Seq_0 IMP_Minus_com IMP_Minus_com nat |
+                      Seq_m IMP_Minus_com IMP_Minus_com nat IMP_Minus_Minus_com  |
+                      Seq_f IMP_Minus_com IMP_Minus_com nat IMP_Minus_Minus_com IMP_Minus_Minus_com  |
+                      If_0  vname IMP_Minus_com IMP_Minus_com nat|
+                      If_m  vname IMP_Minus_com IMP_Minus_com nat IMP_Minus_Minus_com  |
+                      If_f vname IMP_Minus_com IMP_Minus_com nat  IMP_Minus_Minus_com IMP_Minus_Minus_com |
+                      While_0 vname IMP_Minus_com nat|
+                      While_f vname IMP_Minus_com nat IMP_Minus_Minus_com
 
-fun push_on_Stack :: "IMP_Minus_com \<Rightarrow> IMPm_IMPmm list \<Rightarrow> IMPm_IMPmm list" where 
-"push_on_Stack Com.SKIP stack = SKIP # stack "|
-"push_on_Stack (Com.Assign v aexp) stack =  ( Assign v aexp) # stack "|
-"push_on_Stack (Com.Seq c1 c2) stack =  ( Seq_0 c1 c2) # stack "|
-"push_on_Stack (Com.If v c1 c2) stack =  (If_0 v c1 c2) # stack "|
-"push_on_Stack (Com.While v c) stack =  (While_0 v c) # stack "
 
+fun IMPm_IMPmm_encode :: "IMPm_IMPmm \<Rightarrow> nat" where 
+"IMPm_IMPmm_encode (Bot x) = list_encode [0,comm_encode x]"|
+"IMPm_IMPmm_encode (SKIP n) = list_encode [1, n]"|
+"IMPm_IMPmm_encode (Assign v a n) = list_encode [2, vname_encode v, aexp_encode a , n]"|
+"IMPm_IMPmm_encode (Seq_0 c1 c2 n) = list_encode [3, com_encode c1, com_encode c2, n]"|
+"IMPm_IMPmm_encode (Seq_m c1 c2 n c3) = list_encode [4, com_encode c1 ,com_encode c2, n , comm_encode c3]"|
+"IMPm_IMPmm_encode (Seq_f c1 c2 n c3 c4) = list_encode [5, com_encode c1 ,com_encode c2, n , comm_encode c3,comm_encode c4]"|
+"IMPm_IMPmm_encode (If_0 v c1 c2 n) = list_encode [6, vname_encode v, com_encode c1, com_encode c2, n]"|
+"IMPm_IMPmm_encode (If_m v c1 c2 n c3) = list_encode [7, vname_encode v, com_encode c1, com_encode c2, n, comm_encode c3]"|
+"IMPm_IMPmm_encode (If_f v c1 c2 n c3 c4) = list_encode [8, vname_encode v, com_encode c1, com_encode c2, n, comm_encode c3 , comm_encode c4]"|
+"IMPm_IMPmm_encode (While_0 v c n) = list_encode [9, vname_encode v, com_encode c , n]"|
+"IMPm_IMPmm_encode (While_f v c n c') = list_encode [10, vname_encode v, com_encode c, n, comm_encode c']"
+
+fun IMPm_IMPmm_decode :: "nat \<Rightarrow> IMPm_IMPmm" where 
+"IMPm_IMPmm_decode  n = (case list_decode n of
+    [0,x] \<Rightarrow> Bot (comm_decode x)|
+    [Suc 0,n] \<Rightarrow> SKIP n|
+    [Suc (Suc 0) , v , a, n] \<Rightarrow> Assign (vname_decode v) (aexp_decode a) n|
+    [Suc (Suc (Suc 0)), c1, c2,n] \<Rightarrow> Seq_0 (com_decode c1) (com_decode c2) n|
+    [Suc (Suc (Suc (Suc 0))), c1, c2 ,n, c3] \<Rightarrow> Seq_m (com_decode c1) (com_decode c2) n (comm_decode c3)|
+    [Suc (Suc (Suc (Suc (Suc 0)))), c1, c2, n, c3,c4] \<Rightarrow> Seq_f (com_decode c1) (com_decode c2) n (comm_decode c3) (comm_decode c4)|
+    [Suc (Suc (Suc (Suc (Suc (Suc 0))))), v ,c1, c2,n] \<Rightarrow> If_0 (vname_decode v) (com_decode c1)  (com_decode c2) n|
+    [Suc (Suc (Suc (Suc (Suc (Suc (Suc 0)))))), v ,c1 ,c2,n,c3] \<Rightarrow> If_m (vname_decode v) (com_decode c1) (com_decode c2) n (comm_decode c3)|
+    [Suc (Suc (Suc (Suc (Suc (Suc (Suc (Suc 0))))))),v ,c1 ,c2,n,c3,c4] \<Rightarrow> If_f (vname_decode v) (com_decode c1) (com_decode c2) n (comm_decode c3) (comm_decode c4)|
+    [Suc (Suc (Suc (Suc (Suc (Suc (Suc (Suc (Suc 0)))))))),v,c,n] \<Rightarrow> While_0 (vname_decode v) (com_decode c)  n|
+    [Suc (Suc (Suc (Suc (Suc (Suc (Suc (Suc (Suc (Suc 0))))))))), v, c, n, c'] \<Rightarrow> While_f (vname_decode v) (com_decode c) n (comm_decode c')
+) "
+
+lemma IMPm_IMPmm_id : 
+"IMPm_IMPmm_decode (IMPm_IMPmm_encode x) = x"
+  apply(cases x)
+   apply(auto simp add: IMPm_IMPmm_encode.simps IMPm_IMPmm_decode.simps list_encode_inverse comm_id vname_id aexp_id com_id
+                    simp del: comm_encode.simps com_encode.simps comm_decode.simps com_decode.simps aexp_encode.simps aexp_decode.simps)
+  done
+
+definition IMPm_IMPmm_list_encode :: "IMPm_IMPmm list \<Rightarrow> nat" where 
+"IMPm_IMPmm_list_encode xs = list_encode (map IMPm_IMPmm_encode xs)"
+
+definition IMPm_IMPmm_list_decode :: "nat \<Rightarrow> IMPm_IMPmm list " where 
+"IMPm_IMPmm_list_decode xs = map IMPm_IMPmm_decode (list_decode xs)"
+
+lemma IMPm_IMPmm_list_id: 
+"IMPm_IMPmm_list_decode (IMPm_IMPmm_list_encode x) = x"
+  apply(auto simp only:  IMPm_IMPmm_list_decode_def  IMPm_IMPmm_list_encode_def list_encode_inverse 
+            map_map comp_def IMPm_IMPmm_id)
+  apply auto
+  done
+
+fun push_on_stack :: "IMP_Minus_com \<Rightarrow> nat \<Rightarrow> IMPm_IMPmm list \<Rightarrow> IMPm_IMPmm list" where 
+"push_on_stack Com.SKIP n stack = SKIP n # stack "|
+"push_on_stack (Com.Assign v aexp) n stack =  ( Assign v aexp n) # stack "|
+"push_on_stack (Com.Seq c1 c2) n stack =  ( Seq_0 c1 c2 n) # stack "|
+"push_on_stack (Com.If v c1 c2) n stack =  (If_0 v c1 c2 n) # stack "|
+"push_on_stack (Com.While v c) n stack =  (While_0 v c n) # stack "
+
+fun push_on_stack_nat :: "nat \<Rightarrow> nat \<Rightarrow> nat \<Rightarrow> nat" where 
+"push_on_stack_nat c n s = (if hd_nat c = 0 then (1##n##0)##s else 
+if hd_nat c = 1 then (2## (nth_nat (Suc 0) c) ## (nth_nat (Suc (Suc 0)) c) ## n ## 0)## s else 
+if hd_nat c = 2 then (3## (nth_nat (Suc 0) c) ## (nth_nat (Suc (Suc 0)) c) ## n ## 0)## s else 
+if hd_nat c = 3 then (6## (nth_nat (Suc 0) c) ## (nth_nat (Suc (Suc 0)) c) ## (nth_nat (Suc (Suc (Suc 0))) c) ## n ## 0) ## s else
+(9## (nth_nat (Suc 0) c) ## (nth_nat (Suc (Suc 0)) c) ## n ## 0)## s
+)"
+
+lemma sub_push_on_stack:
+"push_on_stack_nat (com_encode c) n (IMPm_IMPmm_list_encode s) = 
+IMPm_IMPmm_list_encode (push_on_stack c n s)"
+  apply(cases c)
+      apply (auto simp only: push_on_stack_nat.simps push_on_stack.simps sub_hd head.simps com_encode.simps
+             IMPm_IMPmm_list_encode_def sub_cons cons0 sub_nth nth.simps)
+  apply auto
+  done
+
+
+
+      
+           
 fun add_result_to_stack :: "IMP_Minus_Minus_com \<Rightarrow> IMPm_IMPmm list \<Rightarrow> IMPm_IMPmm list" where 
-"add_result_to_stack"
+"add_result_to_stack c [] = [Bot c]"|
+"add_result_to_stack c (Seq_0 c1 c2 n # stack) = Seq_m c1 c2 n c # stack" |
+"add_result_to_stack c (Seq_m c1 c2 n c3 #stack) = (Seq_f c1 c2 n c3 c) # stack"|
+"add_result_to_stack c (If_0 v c1 c2  n # stack)  = If_m v c1 c2 n c # stack"|
+"add_result_to_stack c (If_m v c1 c2 n c3 #stack) = If_f v c1 c2 n c3 c # stack"|
+"add_result_to_stack c (While_0 v c' n # stack ) = While_f v c' n c #stack"|
+"add_result_to_stack c s = s"
 
-                      
-fun IMP_Minus_To_IMP_Minus_Minus:: "IMP_Minus_com \<Rightarrow> nat \<Rightarrow> IMP_Minus_Minus_com" where
-"IMP_Minus_To_IMP_Minus_Minus Com.SKIP n = IMP_Minus_Minus_Com.SKIP" |
-"IMP_Minus_To_IMP_Minus_Minus (Com.Assign v aexp) n = assignment_to_binary n v aexp" |
-"IMP_Minus_To_IMP_Minus_Minus (Com.Seq c1 c2) n = 
-  (IMP_Minus_To_IMP_Minus_Minus c1 n ;; IMP_Minus_To_IMP_Minus_Minus c2 n )" |
-"IMP_Minus_To_IMP_Minus_Minus (Com.If v c1 c2) n = (IF (var_bit_list n v)\<noteq>0 THEN
-  IMP_Minus_To_IMP_Minus_Minus c1 n ELSE IMP_Minus_To_IMP_Minus_Minus c2 n)" |
-"IMP_Minus_To_IMP_Minus_Minus (Com.While v c) n = (WHILE (var_bit_list n v)\<noteq>0 DO
-  IMP_Minus_To_IMP_Minus_Minus c n)"
+fun add_result_to_stack_nat :: "nat \<Rightarrow> nat \<Rightarrow> nat" where 
+"add_result_to_stack_nat c s = (if s = 0 then (0##c##0)##0
+else (let h = hd_nat s; con = hd_nat h; t = tl_nat s  in 
+  if con = 3 then ((4## (nth_nat (Suc 0) h) ## (nth_nat (Suc (Suc 0)) h) ## (nth_nat (Suc (Suc (Suc 0))) h) ## c ## 0) ## t) 
+  else if con = 4 then ((5## (nth_nat (Suc 0) h) ## (nth_nat (Suc (Suc 0)) h) ## (nth_nat (Suc (Suc (Suc 0))) h)  ## (nth_nat (Suc (Suc (Suc ( Suc 0)))) h) ## c ## 0) ## t)
+  else if con = 6 then ((7## (nth_nat (Suc 0) h) ## (nth_nat (Suc (Suc 0)) h) ## (nth_nat (Suc (Suc (Suc 0))) h)  ## (nth_nat (Suc (Suc (Suc ( Suc 0)))) h) ## c ## 0) ## t)    
+  else if con = 7 then ((8## (nth_nat (Suc 0) h) ## (nth_nat (Suc (Suc 0)) h) ## (nth_nat (Suc (Suc (Suc 0))) h)  ## (nth_nat (Suc (Suc (Suc ( Suc 0)))) h)  ## (nth_nat (Suc (Suc (Suc ( Suc (Suc 0))))) h) ## c ## 0) ## t)
+  else if con = 9 then ((10 ## (nth_nat (Suc 0) h) ## (nth_nat (Suc (Suc 0)) h) ## (nth_nat (Suc (Suc (Suc 0))) h) ## c ## 0) ## t) 
+  else s
+))"
+
+lemma sub_add_result_to_stack:
+"add_result_to_stack_nat (comm_encode c) (IMPm_IMPmm_list_encode s)
+= IMPm_IMPmm_list_encode (add_result_to_stack c s) "
+  apply(cases s)
+      apply (auto simp only: map_is_Nil_conv
+      list_encode_non_empty  
+      list.simps add_result_to_stack_nat.simps add_result_to_stack.simps sub_hd head.simps comm_encode.simps
+             IMPm_IMPmm_list_encode_def sub_cons cons0 sub_nth nth.simps)
+    
+   apply (auto simp del: list_encode.simps)
+  subgoal for a xs
+    apply(cases a)
+   apply (auto simp add: Let_def sub_tl sub_cons sub_nth sub_hd list.simps simp del: list_encode.simps)
+    done
+  done
+
+function IMP_Minus_to_IMP_Minus_Minus_stack :: "IMPm_IMPmm list \<Rightarrow> IMP_Minus_Minus_com" where 
+"IMP_Minus_to_IMP_Minus_Minus_stack (Seq_0 c1 c2 n #stack) = 
+  IMP_Minus_to_IMP_Minus_Minus_stack (push_on_stack c1 n (Seq_0 c1 c2 n #stack))"|
+"IMP_Minus_to_IMP_Minus_Minus_stack (Seq_m c1 c2 n c3 #stack) = 
+  IMP_Minus_to_IMP_Minus_Minus_stack (push_on_stack c2 n (Seq_m c1 c2 n c3 #stack ))"|
+"IMP_Minus_to_IMP_Minus_Minus_stack (If_0 v c1 c2 n # stack) = 
+  IMP_Minus_to_IMP_Minus_Minus_stack (push_on_stack c1 n (If_0 v c1 c2 n #stack ))"|
+"IMP_Minus_to_IMP_Minus_Minus_stack (If_m v c1 c2 n c3 # stack) = 
+  IMP_Minus_to_IMP_Minus_Minus_stack (push_on_stack c2 n (If_m v c1 c2 n c3 #stack ))"|
+"IMP_Minus_to_IMP_Minus_Minus_stack (While_0 v c n # stack) = 
+  IMP_Minus_to_IMP_Minus_Minus_stack (push_on_stack c n (While_0 v c n #stack ))" |
+"IMP_Minus_to_IMP_Minus_Minus_stack (SKIP _ # stack) = 
+  IMP_Minus_to_IMP_Minus_Minus_stack (add_result_to_stack (IMP_Minus_Minus_Com.SKIP) stack)" |
+"IMP_Minus_to_IMP_Minus_Minus_stack (Assign v aexp n # stack) = 
+  IMP_Minus_to_IMP_Minus_Minus_stack (add_result_to_stack (assignment_to_binary n v aexp) stack)"|
+"IMP_Minus_to_IMP_Minus_Minus_stack (Seq_f _ _ _ c1 c2 # stack) = 
+  IMP_Minus_to_IMP_Minus_Minus_stack (add_result_to_stack (IMP_Minus_Minus_Com.Seq c1 c2) stack)"|
+"IMP_Minus_to_IMP_Minus_Minus_stack (If_f v _ _ n c1 c2 # stack) = 
+  IMP_Minus_to_IMP_Minus_Minus_stack (add_result_to_stack ( IMP_Minus_Minus_Com.If (var_bit_list n v) c1  c2) stack)"|
+"IMP_Minus_to_IMP_Minus_Minus_stack (While_f v _ n c # stack) = 
+  IMP_Minus_to_IMP_Minus_Minus_stack (add_result_to_stack (IMP_Minus_Minus_Com.While (var_bit_list n v) c) stack)"|
+"IMP_Minus_to_IMP_Minus_Minus_stack (Bot res # stack) =  res"
+  sorry
+termination sorry
+
+
+function IMP_Minus_to_IMP_Minus_Minus_stack_nat :: "nat \<Rightarrow> nat" where 
+"IMP_Minus_to_IMP_Minus_Minus_stack_nat s  = ( let h = hd_nat s ; c = hd_nat h ; t = tl_nat s in
+  if c = 3  then  IMP_Minus_to_IMP_Minus_Minus_stack_nat (push_on_stack_nat (nth_nat (Suc 0) h) (nth_nat (Suc (Suc (Suc 0))) h) s)
+else if c = 4 then IMP_Minus_to_IMP_Minus_Minus_stack_nat (push_on_stack_nat (nth_nat (Suc (Suc 0)) h) (nth_nat (Suc (Suc (Suc 0))) h) s) 
+else if c = 6 then IMP_Minus_to_IMP_Minus_Minus_stack_nat (push_on_stack_nat (nth_nat (Suc (Suc 0)) h) (nth_nat (Suc (Suc (Suc (Suc 0)))) h) s)
+else if c = 7 then IMP_Minus_to_IMP_Minus_Minus_stack_nat (push_on_stack_nat (nth_nat (Suc (Suc (Suc 0))) h) (nth_nat (Suc (Suc (Suc (Suc 0)))) h) s)
+else if c = 10 then IMP_Minus_to_IMP_Minus_Minus_stack_nat (push_on_stack_nat (nth_nat (Suc (Suc 0)) h) (nth_nat (Suc (Suc (Suc 0))) h) s) 
+else if c = 1 then IMP_Minus_to_IMP_Minus_Minus_stack_nat (add_result_to_stack_nat (0##0) t)
+else if c = 2 then IMP_Minus_to_IMP_Minus_Minus_stack_nat (add_result_to_stack_nat (assignment_to_binary_nat (nth_nat (Suc (Suc (Suc 0))) h) (nth_nat (Suc 0) h) (nth_nat (Suc (Suc 0)) h)) t)
+else if c = 5 then IMP_Minus_to_IMP_Minus_Minus_stack_nat (add_result_to_stack_nat (2 ## (nth_nat (Suc (Suc (Suc (Suc 0)))) h) ## (nth_nat (Suc (Suc (Suc (Suc 0)))) h) ## 0  ) t) 
+else if c = 8 then IMP_Minus_to_IMP_Minus_Minus_stack_nat (add_result_to_stack_nat (3 ## (var_bit_list_nat (nth_nat (Suc (Suc (Suc (Suc 0)))) h)
+  (nth_nat (Suc 0) h))
+ ## (nth_nat (Suc (Suc (Suc (Suc (Suc 0))))) h) ## (nth_nat (Suc (Suc (Suc (Suc (Suc (Suc 0)))))) h) ## 0  ) t)
+else if c = 10 then IMP_Minus_to_IMP_Minus_Minus_stack_nat (add_result_to_stack_nat (3 ## (var_bit_list_nat (nth_nat (Suc (Suc (Suc 0))) h)
+  (nth_nat (Suc 0) h))
+ ## (nth_nat (Suc (Suc (Suc (Suc 0)))) h)  ## 0  ) t )
+
+else nth_nat (Suc 0) h
+
+)"
+  sorry
+termination sorry
+
+lemma subtailnat_IMP_Minus_to_IMP_Minus_Minus_stack:
+"s \<noteq> []  \<Longrightarrow> IMP_Minus_to_IMP_Minus_Minus_stack_nat (IMPm_IMPmm_list_encode s)
+= comm_encode (IMP_Minus_to_IMP_Minus_Minus_stack s) "
+  apply(induct)
+   apply simp
+  subgoal for a xs
+    apply(cases a)
+   apply(auto simp add: sub_nth Let_def sub_tl sub_add_result_to_stack sub_cons cons0
+  IMPm_IMPmm_list_encode_def sub_hd simp del: push_on_stack_nat.simps add_result_to_stack_nat.simps list_encode.simps )
+    apply(auto simp add: sub_add_result_to_stack simp flip: comm_encode.simps IMPm_IMPmm_list_encode_def  simp del: push_on_stack_nat.simps add_result_to_stack_nat.simps list_encode.simps )
+lemma IMP_Minus_to_IMP_Minus_Minus_stack_correct: 
+"IMP_Minus_to_IMP_Minus_Minus_stack (push_on_stack c n stack) 
+= IMP_Minus_to_IMP_Minus_Minus_stack (add_result_to_stack (IMP_Minus_To_IMP_Minus_Minus c n) stack)"
+  by (induct c arbitrary:stack) auto
+
+definition IMP_Minus_to_IMP_Minus_Minus_tail:: "IMP_Minus_com \<Rightarrow> nat \<Rightarrow> IMP_Minus_Minus_com" where
+  "IMP_Minus_to_IMP_Minus_Minus_tail c n = 
+IMP_Minus_to_IMP_Minus_Minus_stack (push_on_stack c n [])"
+
+lemma subtail_IMP_Minus_to_IMP_Minus_Minus:
+"IMP_Minus_to_IMP_Minus_Minus_tail c n = 
+IMP_Minus_To_IMP_Minus_Minus c n "
+  using  IMP_Minus_to_IMP_Minus_Minus_stack_correct [of c n "[]"]
+  apply (auto simp add:IMP_Minus_to_IMP_Minus_Minus_tail_def)
+  done
+
+
+
 
 fun IMP_Minus_To_IMP_Minus_Minus_nat:: "nat \<Rightarrow> nat \<Rightarrow> nat" where
 "IMP_Minus_To_IMP_Minus_Minus_nat c n = (if c =0 \<or> hd_nat c = 0 then  0##0
